transforms: Complete `Shallow.Map_*` to include all subexpressions

src/Transforms/Shallow.dfy
@@ -11,18 +11,100 @@ module Bootstrap.Transforms.Shallow {
   import opened AST.Predicates
   import opened Generic
 
-  function method {:opaque} Map_Callable(c: Callable, tr: ExprTransformer) : (c': Callable)
-    requires Shallow.All_Callable(c, tr.f.requires)
-    ensures Shallow.All_Callable(c', tr.post) // FIXME Deep
+  function method {:opaque} Map_Module(ent: Module, tr: ExprTransformer) : (ent': Module)
+    requires forall e <- ent.Exprs() :: tr.f.requires(e)
+    ensures forall e <- ent'.Exprs() :: tr.post(e)
   {
-    var req' := Seq.Map(tr.f, c.req);
-    var ens' := Seq.Map(tr.f, c.ens);
-    var body' := c.body.Map(tr.f);
-    match c {
+    Module.Module()
+  }
+
+  function method {:opaque} Map_ExportSet(ent: ExportSet, tr: ExprTransformer) : (ent': ExportSet)
+    requires forall e <- ent.Exprs() :: tr.f.requires(e)
+    ensures forall e <- ent'.Exprs() :: tr.post(e)
+  {
+    ExportSet.ExportSet(provided := ent.provided, revealed := ent.revealed)
+  }
+
+  function method {:opaque} Map_Import(ent: Import, tr: ExprTransformer) : (ent': Import)
+    requires forall e <- ent.Exprs() :: tr.f.requires(e)
+    ensures forall e <- ent'.Exprs() :: tr.post(e)
+  {
+    Import.Import(localName := ent.localName, target := ent.target)
+  }
+
+  function method {:opaque} Map_SubsetType(ent: SubsetType, tr: ExprTransformer) : (ent': SubsetType)
+    requires forall e <- ent.Exprs() :: tr.f.requires(e)
+    ensures forall e <- ent'.Exprs() :: tr.post(e)
+  {
+    SubsetType.SubsetType(
+      boundVar := ent.boundVar, ty := ent.ty, pred := tr.f(ent.pred),
+      witnessExpr := ent.witnessExpr.Map(tr.f), isNewType := ent.isNewType
+    )
+  }
+
+  function method {:opaque} Map_Type(ent: Entities.Type, tr: ExprTransformer) : (ent': Entities.Type)
+    requires forall e <- ent.Exprs() :: tr.f.requires(e)
+    ensures forall e <- ent'.Exprs() :: tr.post(e)
+  {
+    match ent
+      case SubsetType(st) => Entities.Type.SubsetType(Map_SubsetType(st, tr))
+      case TypeAlias(ta) => Entities.Type.TypeAlias(ta)
+      case AbstractType(at) => Entities.Type.AbstractType(at)
+      case TraitType(tt) => Entities.Type.TraitType(tt)
+      case ClassType(ct) => Entities.Type.ClassType(ct)
+      case DataType(dt) => Entities.Type.DataType(dt)
+      case Unsupported(desc) => Entities.Type.Unsupported(desc)
+  }
+
+  function method {:opaque} Map_Field(ent: Field, tr: ExprTransformer) : (ent': Field)
+    requires forall e <- ent.Exprs() :: tr.f.requires(e)
+    ensures forall e <- ent'.Exprs() :: tr.post(e) // FIXME Deep
+  {
+    Field.Field(kind := ent.kind, body := ent.body.Map(tr.f))
+  }
+
+  function method {:opaque} Map_Callable(ent: Callable, tr: ExprTransformer) : (ent': Callable)
+    requires forall e <- ent.Exprs() :: tr.f.requires(e)
+    ensures forall e <- ent'.Exprs() :: tr.post(e) // FIXME Deep
+  {
+    var req' := Seq.Map(tr.f, ent.req);
+    var ens' := Seq.Map(tr.f, ent.ens);
+    var body' := ent.body.Map(tr.f);
+    match ent {
       case Constructor(_, _, _) => Constructor(req', ens', body')
       case Function(_, _, _) => Function(req', ens', body')
       case Method(_, _, _) => Method(req', ens', body')
     }
+  }
+
+  function method {:opaque} Map_Definition(ent: Definition, tr: ExprTransformer) : (ent': Definition)
+    requires forall e <- ent.Exprs() :: tr.f.requires(e)
+    ensures forall e <- ent'.Exprs() :: tr.post(e)
+  {
+    match ent
+      case Field(fi) => Definition.Field(Map_Field(fi, tr))
+      case Callable(ci) => Definition.Callable(Map_Callable(ci, tr))
+  }
+
+  function method {:opaque} Map_Attribute(ent: Attribute, tr: ExprTransformer) : (ent': Attribute)
+    requires forall e <- ent.Exprs() :: tr.f.requires(e)
+    ensures forall e <- ent'.Exprs() :: tr.post(e)
+  {
+    Attribute(name := ent.name, args := Seq.Map(tr.f, ent.args))
+  }
+
+  function method {:opaque} Map_EntityInfo(ent: EntityInfo, tr: ExprTransformer) : (ent': EntityInfo)
+    requires forall e <- ent.Exprs() :: tr.f.requires(e)
+    ensures forall e <- ent'.Exprs() :: tr.post(e)
+    ensures ent'.name == ent.name
+    ensures ent'.members == ent.members
+  {
+    assert forall nm <- ent.members :: nm.ChildOf(ent.name); // BUG: `Valid?`, needed by IDE
+    assert forall a <- ent.attrs, e <- a.Exprs() :: e in ent.Exprs();
+    var ei': EntityInfo := EntityInfo(name := ent.name, location := ent.location,
+      attrs := Seq.Map(a requires a in ent.attrs => Map_Attribute(a, tr), ent.attrs),
+      members := ent.members);
+    ei'
   }
 
   function method {:opaque} Map_Entity(e: Entity, tr: ExprTransformer) : (e': Entity)
@@ -33,12 +115,12 @@ module Bootstrap.Transforms.Shallow {
     ensures e'.ei.members == e.ei.members
   {
     match e {
-      case Definition(ei, d) =>
-        if d.Callable? then
-          Definition(ei, Callable(Map_Callable(d.ci, tr)))
-        else e
-      // TODO: add fields once they contain expressions
-      case _ => e
+      case Module(ei, m) => Entity.Module(Map_EntityInfo(ei, tr), Map_Module(m, tr))
+      case ExportSet(ei, e) => Entity.ExportSet(Map_EntityInfo(ei, tr), Map_ExportSet(e, tr))
+      case Import(ei, i) => Entity.Import(Map_EntityInfo(ei, tr), Map_Import(i, tr))
+      case Type(ei, t) => Entity.Type(Map_EntityInfo(ei, tr), Map_Type(t, tr))
+      case Definition(ei, d) => Entity.Definition(Map_EntityInfo(ei, tr), Map_Definition(d, tr))
+      case Unsupported(ei, desc) => Entity.Unsupported(Map_EntityInfo(ei, tr), desc)
     }
   }
 
@@ -53,12 +135,27 @@ module Bootstrap.Transforms.Shallow {
     assume EntityTransformer?(Map_EntityTransformer(tr));
   }
 
+  function method {:opaque} Map_Registry(r: Registry, tr: ExprTransformer) : (r': Registry)
+    requires forall ent <- r.entities.Values, e <- ent.Exprs() :: tr.f.requires(e)
+    ensures forall ent <- r'.entities.Values, e <- ent.Exprs() :: tr.post(e)
+    ensures r'.MappedFrom?(r)
+  {
+    Map_EntityIsEntityTransformer(tr);
+    r.Map(Map_EntityTransformer(tr))
+  }
+
   function method {:opaque} Map_Program(p: Program, tr: ExprTransformer) : (p': Program)
     requires Shallow.All_Program(p, tr.f.requires)
     ensures Shallow.All_Program(p', tr.post)
   {
-    Map_EntityIsEntityTransformer(tr);
-    var reg' := p.registry.Map(Map_EntityTransformer(tr));
-    Program(reg', defaultModule := p.defaultModule, mainMethod := p.mainMethod)
+    var reg' := Map_Registry(p.registry, tr);
+    var p' := Program(reg', defaultModule := p.defaultModule, mainMethod := p.mainMethod);
+    calc <== {
+      Shallow.All_Program(p', tr.post);
+      forall e <- p'.Exprs() :: tr.post(e);
+      forall ent <- p'.registry.AllRecursiveTransitiveEntities(), e <- ent.Exprs() :: tr.post(e);
+      forall ent <- p'.registry.entities.Values, e <- ent.Exprs() :: tr.post(e);
+    }
+    p'
   }
 }
